rustfrontend/RustIRgenProof.v
@@ -38,12 +38,131 @@ Record match_prog (p : Rustlight.program) (tp : RustIR.program) : Prop := {
     match_prog_types:
     tp.(prog_types) = p.(prog_types);
     match_prog_defs:
-    list_forall2 (fun '(id1, gd) '(id2, tgd) => id1 = id2 /\ match_glob p.(prog_comp_env) gd tgd) p.(prog_defs) tp.(prog_defs);
+    list_forall2 (fun g1 g2 => fst g1 = fst g2 /\ match_glob p.(prog_comp_env) (snd g1) (snd g2)) p.(prog_defs) tp.(prog_defs);
     match_dropm:
     generate_dropm p = RustIR.generate_dropm tp;
     match_prog_skel:
     erase_program tp = erase_program p;
   }.
+
+
+(* Prove match_genv for this specific match_prog *)
+
+Section MATCH_PROGRAMS.
+
+Variable p: program.
+Variable tp: RustIR.program.
+Hypothesis TRANSL: match_prog p tp.
+
+Section INJECT.
+
+Variable j: meminj.
+Variable se: Genv.symtbl.
+Variable tse: Genv.symtbl.
+Hypothesis sematch: Genv.match_stbls j se tse.
+
+Let ce := prog_comp_env p.
+
+Lemma globalenvs_match:
+  Genv.match_genvs j (match_glob ce) (Genv.globalenv se p) (Genv.globalenv tse tp).
+Proof.
+  intros. split; auto. intros. cbn [Genv.globalenv Genv.genv_defs NMap.get].
+  assert (Hd:forall i, Coqlib.option_rel (match_glob ce) (prog_defmap p)!i (prog_defmap tp)!i).
+  {
+    intros.
+    eapply PTree_Properties.of_list_related.
+    apply TRANSL.
+  }
+  rewrite !PTree.fold_spec.
+  apply PTree.elements_canonical_order' in Hd. revert Hd.
+  generalize (prog_defmap p), (prog_defmap tp). intros d1 d2 Hd.
+  (*   cut (option_rel match_gd (PTree.empty _)!b1 (PTree.empty _)!b2). *)
+  cut (Coqlib.option_rel (match_glob ce)
+         (NMap.get _ b1 (NMap.init (option (globdef (Rusttypes.fundef function) type)) None))
+         (NMap.get _ b2 (NMap.init (option (globdef (Rusttypes.fundef RustIR.function) type)) None ))).
+  (* adhoc generalize because types are the same *)
+  - generalize (NMap.init (option (globdef (Rusttypes.fundef function) type)) None).
+    generalize (NMap.init (option (globdef (Rusttypes.fundef RustIR.function) type)) None).
+    induction Hd as [ | [id1 g1] l1 [id2 g2] l2 [Hi Hg] Hl IH]; cbn in *; eauto.
+    intros t1 t2 Ht. eapply IH. eauto. rewrite Hi.
+    eapply Genv.add_globdef_match; eauto.
+  - unfold NMap.get. rewrite !NMap.gi. constructor.
+Qed.
+
+Theorem find_def_match:
+  forall b tb delta g,
+  Genv.find_def (Genv.globalenv se p) b = Some g ->
+  j b = Some (tb, delta) ->
+  exists tg,
+  Genv.find_def (Genv.globalenv tse tp) tb = Some tg /\
+  match_glob ce g tg /\
+  delta = 0.
+Proof.
+  apply Genv.find_def_match_genvs, globalenvs_match.
+Qed.
+
+Theorem find_funct_match:
+  forall v tv f,
+  Genv.find_funct (Genv.globalenv se p) v = Some f ->
+  Val.inject j v tv ->
+  exists tf,
+  Genv.find_funct (Genv.globalenv tse tp) tv = Some tf /\ transl_fundef ce f = tf.
+Proof.
+  intros. exploit Genv.find_funct_inv; eauto. intros [b EQ]. subst v. inv H0.
+  rewrite Genv.find_funct_find_funct_ptr in H. unfold Genv.find_funct_ptr in H.
+  destruct Genv.find_def as [[|]|] eqn:Hf; try congruence. inv H.
+  edestruct find_def_match as (tg & ? & ? & ?); eauto. subst.
+  simpl in H0. destruct tg.
+  rewrite Genv.find_funct_find_funct_ptr. unfold Genv.find_funct_ptr. rewrite H. eauto.
+  contradiction.
+Qed.
+
+
+Theorem find_funct_none:
+  forall v tv,
+  Genv.find_funct (globalenv se p) v = None ->
+  Val.inject j v tv ->
+  v <> Vundef ->
+  Genv.find_funct (RustIR.globalenv tse tp) tv = None.
+Proof.
+  intros v tv Hf1 INJ Hv. destruct INJ; auto; try congruence.
+  destruct (Mem.sup_dec b1 se.(Genv.genv_sup)).
+  - edestruct Genv.mge_dom; eauto. rewrite H1 in H. inv H.
+    rewrite Ptrofs.add_zero. revert Hf1.
+    unfold Genv.find_funct, Genv.find_funct_ptr, Genv.find_def.
+    destruct Ptrofs.eq_dec; auto.
+    generalize (Genv.mge_defs globalenvs_match b1 H1). intros REL. simpl.
+    inv REL. auto.
+    destruct x. congruence. simpl in H2.
+    destruct y. contradiction. auto.    
+  - unfold Genv.find_funct, Genv.find_funct_ptr, Genv.find_def.
+    destruct Ptrofs.eq_dec; auto.
+    destruct NMap.get as [[|]|] eqn:Hdef; auto. exfalso.
+    apply Genv.genv_defs_range in Hdef.
+    eapply Genv.mge_separated in H; eauto. cbn in *.
+    apply n,H,Hdef.
+Qed.
+
+Theorem is_internal_match :
+  (forall f tf, transl_fundef ce f = tf ->
+   fundef_is_internal tf = fundef_is_internal f) ->
+  forall v tv,
+    Val.inject j v tv ->
+    v <> Vundef ->
+    Genv.is_internal (RustIR.globalenv tse tp) tv = Genv.is_internal (globalenv se p) v.
+Proof.
+  intros Hmatch v tv INJ DEF. unfold Genv.is_internal.
+  destruct (Genv.find_funct _ v) eqn:Hf.
+  - edestruct find_funct_match as (tf & Htf & ?); try eassumption.
+    unfold fundef.
+    simpl. setoid_rewrite Htf. eauto.
+  - erewrite find_funct_none; eauto.
+Qed.
+
+
+End INJECT.
+
+End MATCH_PROGRAMS.
 
 
 Section PRESERVATION.
@@ -55,17 +174,71 @@ Variable tprog: RustIR.program.
 Hypothesis TRANSL: match_prog prog tprog.
 
 Variable se: Genv.symtbl.
-Variable tse: Genv.symtbl.
 (* Variable dropflags: PTree.t (list (place * ident)). *)
 
 Let ge := globalenv se prog.
-Let tge := RustIR.globalenv tse tprog.
+Let tge := RustIR.globalenv se tprog.
+
+(* Some lemmas about function definitions in identical symtbls *)
+
+Corollary find_funct_match_id:
+  forall v f,
+  Genv.find_funct ge v = Some f ->
+  exists tf,
+  Genv.find_funct tge v = Some tf /\ transl_fundef ge f = tf.
+Proof.
+  intros. eapply find_funct_match; eauto using Genv.match_stbls_id.
+    apply val_inject_id. auto.
+Qed.
+
+Theorem is_internal_match_id :
+  (forall f tf, transl_fundef ge f = tf ->
+   fundef_is_internal tf = fundef_is_internal f) ->
+  forall v ,
+    v <> Vundef ->
+    Genv.is_internal tge v = Genv.is_internal ge v.
+Proof.
+  intros. destruct v; auto.
+  eapply is_internal_match; eauto using Genv.match_stbls_id.
+  apply val_inject_id; auto. 
+Qed.
+
+
+Lemma comp_env_preserved:
+  RustIR.genv_cenv tge = genv_cenv ge.
+Proof.
+  unfold tge, ge. destruct prog, tprog; simpl. inv TRANSL. simpl in *.
+  congruence.
+Qed.
+
+
+Lemma type_of_fundef_preserved:
+  forall fd tfd,
+  transl_fundef ge fd = tfd -> RustIR.type_of_fundef tfd = type_of_fundef fd.
+Proof.
+  intros. destruct fd; simpl in H; subst.
+  simpl; unfold type_of_function; simpl. auto.
+  simpl; unfold type_of_function; simpl. auto.
+Qed.
+
+Lemma function_not_drop_glue_preserved: forall fd tfd,
+    transl_fundef ge fd = tfd ->
+    function_not_drop_glue fd ->
+    RustIR.function_not_drop_glue tfd.
+Proof.
+  intros. destruct fd.
+  - simpl in *. destruct (fn_drop_glue f) eqn: A; try contradiction.
+    subst. simpl. rewrite A. auto.
+  - subst. simpl in *. auto.
+Qed.
 
 Inductive match_drop_insert_kind: drop_insert_kind -> RustIR.statement -> Prop :=
 | match_drop_reassign: forall p,
     match_drop_insert_kind (drop_reassign p) (gen_drop ge p)
-| match_drop_escape: forall l,
-    match_drop_insert_kind (drop_escape l) (gen_drops_for_escape_vars ge l)
+| match_drop_escape_before: forall l,
+    match_drop_insert_kind (drop_escape_before l) (gen_drops_for_escape_vars ge l)
+| match_drop_escape_after: forall id l,
+    match_drop_insert_kind (drop_escape_after id l) (RustIR.Ssequence (Sstoragedead id) (gen_drops_for_escape_vars ge l))
 | match_drop_return: forall l,
     match_drop_insert_kind (drop_return l) (gen_drops_for_vars ge l)
 | match_drop_reassign_end:
@@ -98,19 +271,23 @@ Inductive match_dropcont : dropcont -> RustIR.statement -> Prop :=
 Inductive match_cont (params: list (ident * type)) : cont -> RustIRown.cont -> Prop :=
 | match_Klet: forall k tk drop id ty
     (MCONT: match_cont params k tk)
-    (DROP: drop = gen_drop ge (Plocal id ty)),
+    (DROP: drop = gen_drops_for_escape_vars ge [(id, ty)]),
     (* when executing Klet, Rustlight would enter Dropinsert state
     where drop_escape contains the out-of-scope variable which is
     related to (drop;storagedead id) *)
-    match_cont params (Klet id ty k) (RustIRown.Kseq (RustIR.Ssequence drop (Sstoragedead id)) tk)
+    (* The additional Kseq is used to simulate the step in Dendlet *)
+    match_cont params (Klet id ty k) (RustIRown.Kseq drop (RustIRown.Kseq RustIR.Sskip tk))
 (* The drops are inserted for the reassignment. The translated
 statement does not contain storagedead *)
 | match_Kdropinsert: forall k tk dk s1 s2 st
     (MCONT: match_cont params k tk)
     (MDCONT: match_dropcont dk s2)
     (MDINS: match_drop_insert_kind st s1),
+    (** TODO: before running st, we may need to execute the
+    storagedead in the target *)
     match_cont params (Kdropinsert st dk k)
-      (RustIRown.Kseq (RustIR.Ssequence s1 s2) tk)
+      (* s1 should contain the storagedead of the first element of st *)
+      (RustIRown.Kseq s1 (RustIRown.Kseq s2 tk))
 | match_Kstop:
     match_cont params Kstop RustIRown.Kstop
 | match_Kseq: forall k s tk ts
@@ -165,22 +342,273 @@ Inductive match_states: Rustlightown.state -> RustIRown.state -> Prop :=
     match_states (Returnstate v k m) (RustIRown.Returnstate v tk m)
 .
 
+Lemma gen_drops_for_escape_vars_nil:
+    gen_drops_for_escape_vars ge nil = RustIR.Sskip.
+Proof.
+  auto.
+Qed.
 
+  
+Lemma gen_drops_for_escape_vars_cons1: forall id ty l,
+    own_type ge ty = true ->
+    gen_drops_for_escape_vars ge ((id, ty) :: l) =
+      RustIR.Ssequence (Sdrop (Plocal id ty)) (RustIR.Ssequence (Sstoragedead id) (gen_drops_for_escape_vars ge l)).
+Proof.
+  unfold gen_drops_for_escape_vars.
+  intros. simpl in *. rewrite H. auto.
+Qed.
+
+
+Lemma gen_drops_for_escape_vars_cons2: forall id ty l,
+    own_type ge ty = false ->
+    gen_drops_for_escape_vars ge ((id, ty) :: l) =
+      RustIR.Ssequence RustIR.Sskip (RustIR.Ssequence (Sstoragedead id) (gen_drops_for_escape_vars ge l)).
+Proof.
+  unfold gen_drops_for_escape_vars.
+  intros. simpl in *. rewrite H.
+ auto.
+Qed.
+
+Lemma gen_drops_for_vars_cons1: forall id ty l,
+    own_type ge ty = true ->
+    gen_drops_for_vars ge ((id, ty) :: l) =
+      RustIR.Ssequence (Sdrop (Plocal id ty)) (gen_drops_for_vars ge l).
+Proof.
+  unfold gen_drops_for_vars.
+  intros. simpl in *.
+  unfold  vars_to_drops. simpl.
+  rewrite H. 
+  auto.
+Qed.
+
+
+Lemma gen_drops_for_vars_cons2: forall id ty l,
+    own_type ge ty = false ->
+    gen_drops_for_vars ge ((id, ty) :: l) =
+      RustIR.Ssequence RustIR.Sskip (gen_drops_for_vars ge l).
+Proof.
+  unfold gen_drops_for_vars.
+  intros. simpl in *.
+  unfold  vars_to_drops. simpl.
+  rewrite H.  
+  auto.
+Qed.
+
+Ltac solve_eval :=
+  try erewrite comp_env_preserved; eauto.
+
+
+Lemma step_in_dropinsert_simulation:
+  forall S1 t S2, step_dropinsert ge S1 t S2 ->
+  forall S1' (MS: match_states S1 S1'), exists S2', plus RustIRown.step tge S1' t S2' /\ match_states S2 S2'.
+Proof.
+  induction 1; intros; inv MS.
+  (* step_dropinsert_to_dropplace_escape *)
+  - inv STMT1. erewrite gen_drops_for_escape_vars_cons1; eauto.
+    eexists. split.
+    (* step *)
+    econstructor.
+    econstructor. eapply star_step.
+    econstructor; eauto. rewrite comp_env_preserved. eauto. 
+    eapply star_refl. 1-2 : eauto.
+    (* match_states *)
+    econstructor; auto.
+    econstructor; auto.
+    econstructor.
+  (* step_dropinsert_to_dropplace_reassign *)
+  - inv STMT1. unfold gen_drop. rewrite OWNTY. simpl.
+    eexists. split.
+    (* step *)
+    econstructor.
+    econstructor. eapply star_step.
+    econstructor; eauto. rewrite comp_env_preserved. eauto. 
+    eapply star_refl. 1-2 : eauto.
+    (* match_states *)
+    econstructor; auto.
+    econstructor; auto.
+    econstructor.
+  (* step_dropinsert_skip_escape *)
+  - inv STMT1. erewrite gen_drops_for_escape_vars_cons2; eauto.
+    eexists. split.
+    (* step *)
+    econstructor.
+    econstructor.
+    eapply star_step. eapply RustIRown.step_skip_seq.
+    eapply star_refl. 1-2: eauto.
+    (* match_states *)
+    econstructor; auto.
+    econstructor; auto.
+  (* step_dropinsert_skip_reassign *)
+  - inv STMT1. unfold gen_drop. rewrite OWNTY. simpl.
+    eexists. split.
+    (* step *)
+    econstructor.
+    econstructor. eapply star_step.
+    econstructor; eauto. 
+    eapply star_refl. 1-2 : eauto.
+    (* match_states *)
+    econstructor; auto.
+    econstructor; auto.
+  (* step_dropinsert_to_dropplace_return *)
+  - inv STMT1. erewrite gen_drops_for_vars_cons1; eauto.
+    eexists. split.
+    (* step *)
+    econstructor.
+    econstructor. eapply star_step.
+    econstructor; eauto.
+    rewrite comp_env_preserved. eauto. 
+    eapply star_refl. 1-2 : eauto.
+    (* match_states *)
+    econstructor; auto.
+    econstructor; auto.
+    econstructor.
+  (* step_dropinsert_skip_return *)
+  - inv STMT1. erewrite gen_drops_for_vars_cons2; eauto.
+    eexists. split.
+    (* step *)
+    econstructor.
+    econstructor. eapply star_step.
+    eapply RustIRown.step_skip_seq.
+    eapply star_refl. 1-2 : eauto.
+    (* match_states *)
+    econstructor; auto.
+    econstructor; auto.
+  (* step_dropinsert_escape_to_after *)
+  - inv STMT1.
+    eexists. split.
+    (* step *)
+    econstructor.
+    econstructor. eapply star_step.
+    econstructor. eapply star_step.
+    eapply RustIRown.step_skip_seq.    
+    eapply star_refl. 1-3 : eauto.
+    (* match_state *)
+    econstructor; auto.
+    constructor.
+  (* step_dropinsert_assign *)
+  - inv STMT1. inv STMT2.
+    eexists. split.
+    econstructor. eapply RustIRown.step_skip_seq.    
+    eapply star_step. econstructor; solve_eval.
+    eapply star_refl. 1-2: eauto.
+    (* match_states *)
+    econstructor; eauto.
+  (* step_dropinsert_assign_variant *)
+  - inv STMT1. inv STMT2.
+    eexists. split.
+    econstructor. eapply RustIRown.step_skip_seq.    
+    eapply star_step. econstructor; solve_eval.
+    eapply star_refl. 1-2: eauto.
+    (* match_states *)
+    econstructor; eauto.
+  (* step_dropinsert_box *)
+  - inv STMT1. inv STMT2.
+    eexists. split.
+    econstructor. eapply RustIRown.step_skip_seq.    
+    eapply star_step. econstructor; solve_eval.
+    eapply star_refl. 1-2: eauto.
+    (* match_states *)
+    econstructor; eauto.
+  (* step_dropinset_call *)
+  - inv STMT1. inv STMT2.
+    exploit find_funct_match_id; eauto.
+    intros (tf & FIND & TRF).
+    eexists. split.
+    econstructor. eapply RustIRown.step_skip_seq.    
+    eapply star_step. econstructor; solve_eval.
+    eapply function_not_drop_glue_preserved; eauto.
+    erewrite type_of_fundef_preserved; eauto.
+    eapply star_refl. 1-2: eauto.
+    (* match_states *)
+    econstructor; eauto.
+    intros. econstructor; auto.
+  (* step_dropinsert_break_seq *)
+  - inv STMT1. inv STMT2. inv MCONT.
+    rewrite gen_drops_for_escape_vars_nil.
+    eexists. split.
+    econstructor. eapply RustIRown.step_skip_seq.
+    eapply star_step. econstructor.
+    eapply star_refl. 1-2: eauto.
+    
+    
 Lemma step_simulation:
   forall S1 t S2, step ge S1 t S2 ->
   forall S1' (MS: match_states S1 S1'), exists S2', plus RustIRown.step tge S1' t S2' /\ match_states S2 S2'.
 Proof.
   induction 1; intros; inv MS.
+  (* step_assign *)
   - simpl.
     eexists. split.
     (* step *)
     econstructor. econstructor.
     eapply star_refl. auto.
     econstructor; auto.
-    unfold gen_drop, gen_drops.
-    destruct (own_type (prog_comp_env prog) (typeof_place p)); auto.
-    econstructor.
-    
+    econstructor. econstructor.
+  (* step_assign_variant *)
+  - simpl.
+    eexists. split.
+    (* step *)
+    econstructor. econstructor.
+    eapply star_refl. auto.
+    econstructor; auto.
+    econstructor. econstructor.
+  (* step_box *)
+  - simpl.
+    eexists. split.
+    (* step *)
+    econstructor. econstructor.
+    eapply star_refl. auto.
+    econstructor; auto.
+    econstructor. econstructor.
+  (* step_let *)
+  - simpl.
+    eexists. split.
+    (* step *)
+    econstructor. econstructor.
+    eapply star_step. econstructor.
+    eapply star_step. econstructor.
+    eapply star_step. econstructor.
+    eapply star_step. econstructor.
+    eapply star_refl. 1-5: eauto.
+    econstructor; auto.
+    econstructor; auto.
+  (* step_end_let *)
+  - simpl. inv MCONT.
+    eexists. split.
+    econstructor. eapply RustIRown.step_skip_seq.
+    eapply star_refl. auto.
+    econstructor; auto.
+    constructor. constructor.
+  (* step_in_dropinsert *)
+  - 
+  (* step_in_dropplace *)
+  - admit.
+  (* step_dropstate *)
+  - admit.
+  (* step_call *)
+  - admit.
+  (* step_internal_function *)
+  - admit.
+  (* step_external_function *)
+  - admit.
+  (* step_return_1 *)
+  - admit.
+  (* step_returnstate *)
+  - admit.
+  (* step_seq *)
+  - admit.
+  (* step_skip_seq *)
+  - admit.
+  (* step_continue_insert_drops *)    
+  - admit.
+  (* step_break_insert_drops *)    
+  - admit.
+  (* step_ifthenelse *)
+  - admit.
+  (* step_loop *)
+  - admit.
+  (* steP_skip_loop *)
+  - admit.
   Admitted. 
 
 (* Theorem transl_program_correct prog tprog:
